src/asn1/RIoT.X509.Extension.fst
@@ -12,10 +12,9 @@ unfold
 let riot_extension_t
 = x509_extension_t OID_RIOT serialize_compositeDeviceID_sequence_TLV
 
-(* ZT: They will fail with rilimit 3 *)
-#set-options "--z3rlimit 8"
-let _ = assert (length_of_oid OID_EC_GRP_SECP256R1 == 6)
-let _ = assert (length_of_asn1_primitive_TLV (Mkbit_string_t 33ul 0ul (magic())) == 35)
+// #set-options "--query_stats --z3rlimit 32 --fuel 8 --ifuel 8"
+// let _ = assert (length_of_oid OID_EC_GRP_SECP256R1 == 6)
+// let _ = assert_norm (length_of_asn1_primitive_TLV (Mkbit_string_t 33ul 0ul (magic())) == 35)
 
 unfold
 let parse_riot_extension
@@ -57,6 +56,31 @@ let lemma_serialize_riot_extension_sequence_TLV_unfold
 let lemma_serialize_riot_extension_sequence_TLV_size
 = lemma_serialize_x509_extension_sequence_TLV_size OID_RIOT serialize_compositeDeviceID_sequence_TLV
 
+#push-options "--query_stats --z3rlimit 64 --fuel 4 --ifuel 4"
+let lemma_serialize_riot_extension_size_exact
+  (x: riot_extension_t_inbound)
+: Lemma (
+  length_of_opaque_serialization serialize_riot_extension x ==
+  length_of_asn1_primitive_TLV x.x509_extValue.riot_version + 109 /\
+  length_of_opaque_serialization serialize_riot_extension x <= 115
+)
+= lemma_serialize_riot_extension_size x;
+  assert (length_of_asn1_primitive_TLV x.x509_extID == 11);
+  lemma_serialize_compositeDeviceID_sequence_TLV_size_exact x.x509_extValue;
+  assert (length_of_TLV OCTET_STRING (length_of_opaque_serialization serialize_compositeDeviceID_sequence_TLV x.x509_extValue)
+          == length_of_asn1_primitive_TLV x.x509_extValue.riot_version + 95)
+
+let lemma_serialize_riot_extension_sequence_TLV_size_exact
+  (x: riot_extension_t_inbound)
+: Lemma (
+  length_of_opaque_serialization serialize_riot_extension_sequence_TLV x ==
+  length_of_asn1_primitive_TLV x.x509_extValue.riot_version + 111 /\
+  length_of_opaque_serialization serialize_riot_extension x <= 117
+)
+= lemma_serialize_riot_extension_sequence_TLV_size x;
+  lemma_serialize_riot_extension_size_exact x
+#pop-options
+
 (* low *)
 open ASN1.Low
 
@@ -78,6 +102,33 @@ let serialize32_riot_extension_sequence_TLV_backwards
   (* prf*) ()
 
 
-#set-options "--z3rlimit 8"
-let _ = assert (length_of_oid OID_EC_GRP_SECP256R1 == 6)
-let _ = assert (length_of_asn1_primitive_TLV (Mkbit_string_t 33ul 0ul (magic())) == 35)
+// #set-options "--z3rlimit 8"
+// let _ = assert (length_of_oid OID_EC_GRP_SECP256R1 == 6)
+// let _ = assert (length_of_asn1_primitive_TLV (Mkbit_string_t 33ul 0ul (magic())) == 35)
+
+(* helpers *)
+module B32 = FStar.Bytes
+
+#restart-solver
+#push-options "--query_stats --z3rlimit 64 --fuel 8 --ifuel 4"
+let x509_get_riot_extension
+  (version: datatype_of_asn1_type INTEGER)
+  (deviceKeyPub: B32.lbytes32 32ul)
+  (fwid: B32.lbytes32 32ul)
+: Tot (riot_extension_t_inbound)
+=
+  let compositeDeviceID: compositeDeviceID_t_inbound = x509_get_compositeDeviceID version deviceKeyPub fwid in
+  (* Prf *) lemma_serialize_compositeDeviceID_sequence_TLV_size_exact compositeDeviceID;
+
+  let riot_extension: riot_extension_t = {
+    x509_extID       = OID_RIOT;
+    x509_extCritical = false;
+    x509_extValue    = compositeDeviceID
+  } in
+  (* Prf *) lemma_serialize_riot_extension_unfold riot_extension;
+  (* Prf *) lemma_serialize_riot_extension_size   riot_extension;
+  (* Prf *) (**) lemma_serialize_asn1_oid_TLV_size riot_extension.x509_extID;
+  (* Prf *) (**) lemma_serialize_asn1_boolean_TLV_size riot_extension.x509_extCritical;
+
+(*return*) riot_extension
+#pop-options
