src/asn1/RIoT.Declassify.fsti
@@ -10,19 +10,19 @@ module B32 = FStar.Bytes
 
 noextract
 val declassify_secret_bytes
-  (l: nat)
-  (sec: Seq.lseq uint8 l)
-: GTot (pub: Seq.lseq pub_uint8 l
-          { forall (i:nat{i < l}).
-              v (Seq.index sec i) == v (Seq.index pub i) })
+  (sec: Seq.seq uint8)
+: GTot (pub: Seq.seq pub_uint8
+          { Seq.length sec == Seq.length pub /\
+            (forall (i:nat{i < Seq.length pub}).
+              v (Seq.index sec i) == v (Seq.index pub i)) })
 
 noextract
 val classify_public_bytes
-  (l: nat)
-  (pub: Seq.lseq pub_uint8 l)
-: GTot (sec: Seq.lseq uint8 l
-          { forall (i:nat{i < l}).
-              v (Seq.index sec i) == v (Seq.index pub i) })
+  (pub: Seq.seq pub_uint8)
+: GTot (sec: Seq.seq uint8
+          { Seq.length sec == Seq.length pub /\
+            (forall (i:nat{i < Seq.length pub}).
+              v (Seq.index sec i) == v (Seq.index pub i)) })
 
 val declassify_secret_buffer
   (len: size_t)
@@ -34,7 +34,7 @@ val declassify_secret_buffer
     B.disjoint src dst)
   (ensures fun h0 _ h1 ->
     B.(modifies (loc_buffer dst) h0 h1) /\
-    B.as_seq h1 dst == declassify_secret_bytes (v len) (B.as_seq h1 src))
+    B.as_seq h1 dst == declassify_secret_bytes (B.as_seq h1 src))
 
 val classify_public_buffer
   (len: size_t)
@@ -46,4 +46,4 @@ val classify_public_buffer
     B.disjoint src dst)
   (ensures fun h0 _ h1 ->
     B.(modifies (loc_buffer dst) h0 h1) /\
-    B.as_seq h1 dst == classify_public_bytes (v len) (B.as_seq h1 src))
+    B.as_seq h1 dst == classify_public_bytes (B.as_seq h1 src))
