src/asn1/X509.Crypto.Signature.fst
@@ -13,10 +13,26 @@ module B32 = FStar.Bytes
 
 open ASN1.Base
 
-let x509_signature_t
+let x509_signature_t_aux
   (alg: cryptoAlg {alg == ED25519})
 = match alg with
   | ED25519   -> datatype_of_asn1_type BIT_STRING
+
+let filter_x509_signature
+  (alg: cryptoAlg {alg == ED25519})
+  (x: x509_signature_t_aux alg)
+: GTot (bool)
+= match alg with
+  | ED25519   -> ( let x = x <: datatype_of_asn1_type BIT_STRING in
+                   x.bs_len = 65ul &&
+                   x.bs_unused_bits = 0ul )
+
+let x509_signature_t
+  (alg: cryptoAlg {alg == ED25519})
+= match alg with
+  | ED25519   -> ( bs: datatype_of_asn1_type BIT_STRING
+                       { v bs.bs_len == 65 /\
+                         v bs.bs_unused_bits == 0 })
 
 let parse_x509_signature_kind
   (alg: cryptoAlg {alg == ED25519})
@@ -27,13 +43,59 @@ let parse_x509_signature
   (alg: cryptoAlg {alg == ED25519})
 : parser (parse_x509_signature_kind alg) (x509_signature_t alg)
 = match alg with
-  | ED25519   -> ( parse_asn1_TLV_of_type BIT_STRING )
+  | ED25519   -> ( parse_asn1_TLV_of_type BIT_STRING
+                   `parse_filter`
+                   filter_x509_signature alg
+                   `parse_synth`
+                   (fun x -> x <: x509_signature_t alg))
 
 let serialize_x509_signature
   (alg: cryptoAlg {alg == ED25519})
 : serializer (parse_x509_signature alg)
 = match alg with
-  | ED25519   -> ( serialize_asn1_TLV_of_type BIT_STRING )
+  | ED25519   -> ( serialize_synth
+                   (* p1 *) (parse_asn1_TLV_of_type BIT_STRING
+                             `parse_filter`
+                             filter_x509_signature alg)
+                   (* f2 *) (fun x -> x <: x509_signature_t alg)
+                   (* s1 *) (serialize_asn1_TLV_of_type BIT_STRING
+                             `serialize_filter`
+                             filter_x509_signature alg)
+                   (* g1 *) (fun x -> x <: parse_filter_refine (filter_x509_signature alg))
+                   (* prf*) () )
+
+let lemma_serialize_x509_signature_unfold
+  (alg: cryptoAlg {alg == ED25519})
+  (x: x509_signature_t alg)
+: Lemma (
+  match alg with
+  | ED25519   -> ( serialize_x509_signature alg `serialize` x ==
+                   serialize_asn1_TLV_of_type BIT_STRING x )
+)
+= serialize_synth_eq
+  (* p1 *) (parse_asn1_TLV_of_type BIT_STRING
+            `parse_filter`
+            filter_x509_signature alg)
+  (* f2 *) (fun x -> x <: x509_signature_t alg)
+  (* s1 *) (serialize_asn1_TLV_of_type BIT_STRING
+            `serialize_filter`
+            filter_x509_signature alg)
+  (* g1 *) (fun x -> x <: parse_filter_refine (filter_x509_signature alg))
+  (* prf*) ()
+  (* in *) x
+
+let lemma_serialize_x509_signature_size
+  (alg: cryptoAlg {alg == ED25519})
+  (x: x509_signature_t alg)
+: Lemma (
+  match alg with
+  | ED25519   -> ( length_of_opaque_serialization (serialize_x509_signature alg) x ==
+                   length_of_asn1_primitive_TLV #BIT_STRING x /\
+                   length_of_opaque_serialization (serialize_x509_signature alg) x == 67 )
+)
+= match alg with
+  | ED25519   -> ( lemma_serialize_x509_signature_unfold alg x;
+                   lemma_serialize_asn1_bit_string_TLV_size x )
 
 let x509_signature_t_inbound
   (alg: cryptoAlg {alg == ED25519})
@@ -66,15 +128,55 @@ let lemma_serialize_x509_signature_sequence_TLV_size
 = match alg with
   | ED25519   -> ( lemma_serialize_asn1_sequence_TLV_size (serialize_x509_signature alg) x )
 
+#push-options "--z3rlimit 32 --fuel 4 --ifuel 4"
+let lemma_serialize_x509_signature_sequence_TLV_size_exact
+  (alg: cryptoAlg {alg == ED25519})
+  (x: x509_signature_t_inbound alg)
+: Lemma (
+  match alg with
+  | ED25519    -> ( length_of_opaque_serialization (serialize_x509_signature_sequence_TLV alg) x == 69 )
+)
+= match alg with
+  | ED25519    -> ( lemma_serialize_x509_signature_sequence_TLV_size alg x;
+                    lemma_serialize_x509_signature_size alg x )
+#pop-options
+
 (* Low *)
 let serialize32_x509_signature_backwards
   (alg: cryptoAlg {alg == ED25519})
 : serializer32_backwards (serialize_x509_signature alg)
 = match alg with
-  | ED25519   -> ( serialize32_asn1_bit_string_TLV_backwards () )
+  | ED25519   -> ( serialize32_synth_backwards
+                   (* s32 *) (serialize32_asn1_bit_string_TLV_backwards ()
+                              `serialize32_filter_backwards`
+                              filter_x509_signature alg)
+                   (* f2  *) (fun x -> x <: x509_signature_t alg)
+                   (* g1  *) (fun x -> x <: parse_filter_refine (filter_x509_signature alg))
+                   (* g1' *) (fun x -> x <: parse_filter_refine (filter_x509_signature alg))
+                   (* prf *) () )
 
 let serialize32_x509_signature_sequence_TLV_backwards
   (alg: cryptoAlg {alg == ED25519})
 : serializer32_backwards (serialize_x509_signature_sequence_TLV alg)
 = match alg with
   | ED25519   -> ( serialize32_asn1_sequence_TLV_backwards (serialize32_x509_signature_backwards alg) )
+
+
+(* Helpers *)
+let _ = assert (length_of_oid OID_EC_GRP_SECP256R1 == 6)
+
+module B32 = FStar.Bytes
+let x509_signature_raw_t
+  (alg: cryptoAlg {alg == ED25519})
+= match alg with
+  | ED25519   -> ( B32.lbytes32 64ul )
+
+let x509_get_signature
+  (alg: cryptoAlg {alg == ED25519})
+  (sig32: x509_signature_raw_t alg)
+: Tot (x509_signature_t_inbound alg)
+=
+  match alg with
+  | ED25519   -> ( let sig_bs: x509_signature_t alg = Mkbit_string_t 65ul 0ul sig32 in
+                   (* Prf *) lemma_serialize_x509_signature_size alg sig_bs;
+                   (* return *) sig_bs )
